Tap

DLCF/Typing/Basic.lean
@@ -11,26 +11,33 @@ namespace Term
 inductive JEq : Finset FVar → Term → Term → Term → Prop
   | nil_ok : JEq ∅ ⊤ .nil .nil
   | cons_ok (hA : JEq Γ (.univ n) A A) : JEq (insert ⟨i, A⟩ Γ) ⊤ .nil .nil
-  | var (hΓ : JEq Γ ⊤ .nil .nil) (hx : ⟨i, A⟩ ∈ Γ) : JEq Γ A (.free i A) (.free i A)
+  | var (hΓ : JEq Γ (.univ n) A A) (hx : ⟨i, A⟩ ∈ Γ) : JEq Γ A (.free i A) (.free i A)
   | top (hΓ : JEq Γ ⊤ .nil .nil) : JEq Γ (.univ 0) .top .top
   | bot (hΓ : JEq Γ ⊤ .nil .nil) : JEq Γ (.univ 0) .bot .bot
   | univ (hΓ : JEq Γ ⊤ .nil .nil) : JEq Γ (.univ (n + 1)) (.univ n) (.univ n)
   -- TODO: swap from cofinite quantification to universal?
-  | pi (L : Finset FVar) (x) (hx : x ∉ L)
+  | pi
     (hA : JEq Γ (.univ n) A A')
-    (hB : JEq (insert x Γ) (.univ m) (b0 x • B) (b0 x • B'))
+    (hx : ⟨i, A⟩ ∉ Γ ∪ fv B)
+    (hB : JEq (insert ⟨i, A⟩ Γ) (.univ m) (b0 (.free i A) • B) (b0 (.free i A) • B'))
     : JEq Γ (.univ (imax n m)) (.pi A B) (.pi A' B')
   | app (hf : JEq Γ (.pi A B) f f') (ha : JEq Γ A a a') : JEq Γ (b0 a • B) (.app f a) (.app f' a')
-  | abs (L : Finset FVar) (x) (hx : x ∉ L)
+  | abs
     (hA : JEq Γ (.univ n) A A')
-    (ht : JEq (insert x Γ) (b0 x • B) (b0 x • t) (b0 x • t'))
+    (hx : ⟨i, A⟩ ∉ Γ ∪ fv t)
+    (ht : JEq (insert ⟨i, A⟩ Γ) (b0 (.free i A) • B) (b0 (.free i A) • t) (b0 (.free i A) • t'))
     : JEq Γ (.pi A B) (.abs A t) (.abs A' t')
   | eq
     (hA : JEq Γ (.univ n) A A')
     (ha : JEq Γ A a a')
-    (hb : JEq Γ A' b b')
+    (hb : JEq Γ A b b')
     : JEq Γ (.univ 0) (.eq A a b) (.eq A' a' b')
   | eq_rfl (jab : JEq Γ A a b) : JEq Γ (.eq A a b) .nil .nil
+  -- β-reduction
+  | β_abs
+    (h : JEq Γ B l (.app (.abs A t) r)) : JEq Γ B l (b0 r • t)
+  -- η-expansion
+  | η_abs (h : JEq Γ (.pi A B) l r) : JEq Γ (.pi A B) l (.abs A (.app r (.bound 0)))
   -- Extensionality
   | jeq_ext (eab : JEq Γ (.eq A a b) .nil .nil) : JEq Γ A a b
   -- Propositional extensionality
@@ -43,6 +50,7 @@ inductive JEq : Finset FVar → Term → Term → Term → Prop
   -- Propositional irrelevance
   | u0_irr (hA : JEq Γ (.univ 0) A A) (ha : JEq Γ A a a) : JEq Γ A a .nil
   -- Double negation elimination
+  -- TODO: generalize to truncation elimination
   | dne (hA : JEq Γ (.univ 0) A A) (hna : JEq Γ (.neg (.neg A)) .nil .nil) : JEq Γ A .nil .nil
   -- The axiom of choice
   | aoc (hf : JEq Γ (.pi A (.trunc B)) .nil .nil) : JEq Γ (.trunc (.pi A B)) .nil .nil
@@ -50,43 +58,168 @@ inductive JEq : Finset FVar → Term → Term → Term → Prop
   | cast : JEq Γ (.univ n) A B → JEq Γ A a b → JEq Γ B a b
   | trans : JEq Γ A a b → JEq Γ A b c → JEq Γ A a c
 
+attribute [simp] JEq.nil_ok
+
 notation Γ " ⊢ " a " ≡ " b " : " A => JEq Γ A a b
 
-notation Γ " ⊢ " a " : " A => Γ ⊢ a ≡ a : A
-
-notation Γ " ok" => Γ ⊢ Term.nil : ⊤
-
-theorem JEq.cons_ok' (x : FVar) (hA : Γ ⊢ x.ty : .univ n) : (insert x Γ) ok
-  := by cases x; exact .cons_ok hA
-
-theorem JEq.u0_jeq (hA : Γ ⊢ A : .univ 0) (hp : Γ ⊢ p : A) (hq : Γ ⊢ q : A) : Γ ⊢ p ≡ q : A
-  := .trans (.u0_irr hA hp) (.symm (.u0_irr hA hq))
-
-theorem JEq.ctx_ok (h : Γ ⊢ a ≡ b : A) : Γ ok := by induction h with
+theorem JEq.to_nil (h : Γ ⊢ a ≡ b : A) : Γ ⊢ .nil ≡ .nil : ⊤ := by induction h with
   | nil_ok => exact .nil_ok
   | cons_ok hA => exact .cons_ok hA
   | _ => assumption
 
--- TODO: existential introduction rules
+-- notation Γ " ok" => Γ ⊢ Term.nil : ⊤
 
--- TODO: universal elimination rules (?)
+inductive HasTy : Finset FVar → Term → Term → Prop
+  | nil_ok : HasTy ∅ ⊤ .nil
+  | cons_ok (hA : HasTy Γ (.univ n) A) : HasTy (insert ⟨i, A⟩ Γ) ⊤ .nil
+  | var (hΓ : HasTy Γ (.univ n) A) (hx : ⟨i, A⟩ ∈ Γ) : HasTy Γ A (.free i A)
+  | top (hΓ : HasTy Γ ⊤ .nil) : HasTy Γ (.univ 0) ⊤
+  | bot (hΓ : HasTy Γ ⊤ .nil) : HasTy Γ (.univ 0) .bot
+  | univ (hΓ : HasTy Γ ⊤ .nil) : HasTy Γ (.univ (n + 1)) (.univ n)
+  | pi
+    (hA : HasTy Γ (.univ n) A)
+    (hx : ⟨i, A⟩ ∉ Γ ∪ fv B)
+    (hB : HasTy (insert ⟨i, A⟩ Γ) (.univ m) (b0 (.free i A) • B))
+    : HasTy Γ (.univ (imax n m)) (.pi A B)
+  | app (hf : HasTy Γ (.pi A B) f) (ha : HasTy Γ A a) : HasTy Γ (b0 a • B) (.app f a)
+  | abs
+    (hA : HasTy Γ (.univ n) A)
+    (hx : ⟨i, A⟩ ∉ Γ ∪ fv t)
+    (ht : HasTy (insert ⟨i, A⟩ Γ) (b0 (.free i A) • B) (b0 (.free i A) • t))
+    : HasTy Γ (.pi A B) (.abs A t)
+  | eq
+    (hA : HasTy Γ (.univ n) A)
+    (ha : HasTy Γ A a)
+    (hb : HasTy Γ A b)
+    : HasTy Γ (.univ 0) (.eq A a b)
+  | eq_rfl (h : Γ ⊢ a ≡ b : A) : HasTy Γ (.eq A a b) .nil
+  | cast (h : Γ ⊢ A ≡ B : .univ n) (ha : HasTy Γ A a) : HasTy Γ B a
 
--- TODO: lore about universes, regularity, and other such nonsense
+notation Γ " ⊢ " a " : " A => HasTy Γ A a
 
-abbrev Wf (Γ : Finset FVar) (A : Term) := {t : Term // Γ ⊢ t : A}
+theorem HasTy.refl {Γ A a} (h : Γ ⊢ a : A) : Γ ⊢ a ≡ a : A := by induction h with
+  | cast h ha Ia => exact .cast h Ia
+  | _ => constructor <;> (try apply JEq.to_nil) <;> assumption
 
-instance Wf.setoid (Γ : Finset FVar) (A : Term) : Setoid (Term.Wf Γ A) where
-  r s t := Γ ⊢ s.val ≡ t.val : A
-  iseqv := {
-    refl x := x.prop,
-    symm h := .symm h,
-    trans h h' := .trans h h'
-  }
+-- theorem JEq.left_eq_helper {Γ A a} (h : Γ ⊢ a ≡ b : A) (hab : a = b) : Γ ⊢ a : A := by
+--   induction h with
+--   | β_abs => sorry -- TODO: needs inversion + substitution
+--   | η_abs => sorry
+--   | jeq_ext => sorry
+--   | u0_ext => sorry
+--   | u0_irr => sorry
+--   | dne => sorry
+--   | aoc => sorry
+--   | symm => sorry
+--   | cast => sorry
+--   | trans => sorry
+--   | _ => cases hab; constructor <;> apply_assumption <;> rfl
 
--- TODO: constructors for Wf
+-- theorem JEq.left {Γ A a} (h : Γ ⊢ a ≡ b : A) : Γ ⊢ a : A := by
+  -- induction h with
+  -- | pi => sorry
+  -- | abs => sorry
+  -- | app => sorry
+  -- | eq hA ha hb IA Ia Ib => exact ⟨.eq IA.left Ia.left Ib.left, .eq IA.right (Ia.left.cast IA) sorry⟩
+  -- | eq_rfl => sorry
+  -- | β_abs => sorry
+  -- | η_abs => sorry
+  -- | jeq_ext => sorry
+  -- | u0_ext => sorry
+  -- | u0_irr => sorry
+  -- | dne => sorry
+  -- | aoc => sorry
+  -- | symm => sorry
+  -- | cast => sorry
+  -- | trans => sorry
+  -- | _ =>
+  --   (try casesm* _ ∧ _)
+  --   constructor
+  --   · constructor <;> assumption
+  --   · constructor <;> assumption
 
--- TODO: congruence theorems for Wf
+-- inductive CtxOk : Finset FVar → Prop
+--   | nil_ok : CtxOk ∅
+--   | cons_ok {Γ i A} (hΓ : CtxOk Γ) (hA : Γ ⊢ A : .univ n) : CtxOk (insert ⟨i, A⟩ Γ)
 
-abbrev Eqv (Γ : Finset FVar) (A : Term) := Quotient (Wf.setoid Γ A)
+-- attribute [simp] CtxOk.nil_ok
+
+-- theorem CtxOk.jeq_nil {Γ} (hΓ : CtxOk Γ) : Γ ⊢ .nil : ⊤ := by induction hΓ with
+--   | nil_ok => exact .nil_ok
+--   | cons_ok hΓ hA => exact .cons_ok hA
+
+-- theorem CtxOk.of_jeq_nil {Γ} (hΓ : Γ ⊢ .nil : ⊤) : CtxOk Γ := by
+--   generalize ht : (⊤ : Term) = t at hΓ
+--   generalize hn : Term.nil = n at hΓ
+--   sorry
+
+-- theorem CtxOk.iff_jeq_nil {Γ} : CtxOk Γ ↔ Γ ⊢ .nil : ⊤ := by induction Γ using Finset.induction with
+--   | empty => simp
+--   | insert hx Ih =>
+--     rename_i x Γ
+--     cases x with | mk i A =>
+--     constructor
+--     · intro hΓ
+--       sorry
+--     · sorry
+
+-- theorem JEq.left_wf (h : Γ ⊢ a ≡ b : A) : Γ ⊢ a : A := .trans h (.symm h)
+
+-- theorem JEq.right_wf (h : Γ ⊢ a ≡ b : A) : Γ ⊢ b : A := .trans (.symm h) h
+
+-- theorem JEq.cons_ok' (x : FVar) (hA : Γ ⊢ x.ty : .univ n) : (insert x Γ) ok
+--   := by cases x; exact .cons_ok hA
+
+-- theorem JEq.u0_jeq (hA : Γ ⊢ A : .univ 0) (hp : Γ ⊢ p : A) (hq : Γ ⊢ q : A) : Γ ⊢ p ≡ q : A
+--   := .trans (.u0_irr hA hp) (.symm (.u0_irr hA hq))
+
+
+-- def IsTy (Γ : Finset FVar) (A : Term) := ∃n, Γ ⊢ A : .univ n
+
+-- notation Γ " ⊢ " A " isty" => IsTy Γ A
+
+-- theorem IsTy.top {Γ : Finset FVar} (h : Γ ok) : Γ ⊢ .top isty := ⟨0, .top h⟩
+
+-- theorem IsTy.bot {Γ : Finset FVar} (h : Γ ok) : Γ ⊢ .bot isty := ⟨0, .bot h⟩
+
+-- theorem IsTy.univ {n} {Γ : Finset FVar} (h : Γ ok) : Γ ⊢ .univ n isty := ⟨n + 1, .univ h⟩
+
+-- theorem IsTy.pi {Γ : Finset FVar} {A B}
+--    (hA : Γ ⊢ A isty)
+--    (hx : ⟨i, A⟩ ∉ Γ ∪ fv B)
+--    (hB : insert ⟨i, A⟩ Γ ⊢ b0 (.free i A) • B isty)
+--   : Γ ⊢ .pi A B isty
+--   := have ⟨_, hA⟩ := hA; have ⟨_, hB⟩ := hB; ⟨_, .pi hA hx hB⟩
+
+-- @[match_pattern]
+-- theorem IsTy.eq {Γ : Finset FVar} {A a b} (hA : Γ ⊢ A isty) (ha : Γ ⊢ a : A) (hb : Γ ⊢ b : A)
+--   : Γ ⊢ .eq A a b isty := have ⟨_, hA⟩ := hA; ⟨0, .eq hA ha hb⟩
+
+-- theorem JEq.regular (h : Γ ⊢ a ≡ b : A) : Γ ⊢ A isty := by induction h with
+--   | nil_ok => exact .top .nil_ok
+--   | cons_ok hA => exact .top (.cons_ok hA)
+--   | _ => sorry
+
+-- -- TODO: existential introduction rules
+
+-- -- TODO: universal elimination rules (?)
+
+-- -- TODO: lore about universes, regularity, and other such nonsense
+
+-- abbrev Wf (Γ : Finset FVar) (A : Term) := {t : Term // Γ ⊢ t : A}
+
+-- instance Wf.setoid (Γ : Finset FVar) (A : Term) : Setoid (Term.Wf Γ A) where
+--   r s t := Γ ⊢ s.val ≡ t.val : A
+--   iseqv := {
+--     refl x := x.prop,
+--     symm h := .symm h,
+--     trans h h' := .trans h h'
+--   }
+
+-- -- TODO: constructors for Wf
+
+-- -- TODO: congruence theorems for Wf
+
+-- abbrev Eqv (Γ : Finset FVar) (A : Term) := Quotient (Wf.setoid Γ A)
 
 -- TODO: constructors for Eqv
